HM_Theorems.thy
@@ -1,0 +1,167 @@
+theory HM_Theorems
+imports Main HML_list
+begin
+
+context lts
+begin
+
+section \<open>Hennessy-Milner Theorem of the Trace Modal Logic subset and Trace-equivalence\<close>
+
+text \<open>HM-trace Theorem should follow from this:\<close>
+
+lemma ttf:
+  fixes p t
+  shows "t \<in> traces p = (p \<Turnstile> trace_to_formula t)"
+proof
+  define \<phi> where "\<phi> = trace_to_formula t"
+  assume "t \<in> traces p"
+  show "p \<Turnstile> trace_to_formula t"
+    using \<open>t \<in> traces p\<close>
+  proof(induction t arbitrary: p)
+    case Nil
+    then show ?case by simp
+  next
+    case (Cons a t)
+    from Cons obtain p'' p' where "p'' \<mapsto>$ t p'" "p \<mapsto>a p''" 
+      using step_sequence.simps list.distinct(1) list.sel(1) list.sel(3)
+      by (smt (verit) mem_Collect_eq)
+    then show ?case using trace_to_formula.simps HML_semantics.cases Cons
+      by fastforce
+    qed
+next
+  assume "p \<Turnstile> trace_to_formula t"
+  show "t \<in> traces p"
+    using \<open>p \<Turnstile> trace_to_formula t\<close>
+  proof(induction t arbitrary: p)
+    case Nil
+    then show ?case 
+      using step_sequence.intros(1) by fastforce
+  next
+    case (Cons a t)
+    from Cons obtain p' where p'sat: "p \<mapsto>a p'" "p' \<Turnstile> (trace_to_formula t)" by auto
+    with Cons(1) have "t \<in> traces p'" by simp
+    with \<open>p \<mapsto>a p'\<close> show ?case
+      using step_sequence.intros(2) by fastforce
+  qed
+qed
+
+lemma ttf_in_HML_trace:
+  fixes t
+  shows "(trace_to_formula t) \<in> HML_trace_formulas"
+ proof(induction t)
+  case Nil
+  then show ?case 
+    by (simp add: HML_trace_formulas_def trace_conj)
+next
+  case (Cons a t)
+  then show ?case
+    by (simp add: HML_trace_formulas_def trace_pos)
+qed
+
+lemma HM_trace_aux_theorem:
+  fixes p \<phi>
+  assumes "(\<phi> \<in> HML_trace_formulas \<and> (p \<Turnstile> \<phi>))"  
+  shows "\<exists>t. t \<in> traces p \<and> (\<phi> = (trace_to_formula t))"
+  using assms
+proof(induction \<phi> arbitrary: p)
+  case (HML_conj x1 x2)
+  then have "x1 = [] \<and> x2 = []"
+    using HML_trace.simps HML_trace_formulas_def formula_list.simps(4) by blast
+  then show ?case
+    using step_sequence.intros(1) by fastforce
+next
+  case (HML_poss \<alpha> \<phi>)  
+  then have \<phi>_trace: "\<phi> \<in> HML_trace_formulas"
+    using HML_trace.simps HML_trace_formulas_def by fastforce
+  from HML_poss HML_sem_poss obtain q where "p \<mapsto>\<alpha> q \<and> q \<Turnstile> \<phi>"
+    by blast
+  with HML_poss \<phi>_trace have "\<exists>t. t \<in> traces q \<and> \<phi> = trace_to_formula t" by blast
+  then show ?case 
+    using \<open>p \<mapsto>\<alpha> q \<and> q \<Turnstile> \<phi>\<close> step_sequence.intros(2) by fastforce
+qed
+
+lemma state_satisfies_trace:
+  fixes p t
+  assumes "t \<in> traces p"
+  shows "p \<Turnstile> trace_to_formula t"
+  using \<open>t \<in> traces p\<close>
+proof(induction t arbitrary: p)
+  case Nil
+  then show ?case
+    by simp
+next
+  case (Cons a t)
+  with trace_to_formula.simps(2) show ?case
+    by (smt (verit, best) formula_list.distinct(1) list.inject local.HML_sem_poss mem_Collect_eq step_sequence.cases trace_to_formula.simps(1))
+qed
+
+text \<open>HM Theorem for Traces\<close>
+
+lemma HM_trace_theorem:
+  fixes p q
+  shows "(traces p = traces q) = 
+(\<forall>\<phi>. \<phi> \<in> HML_trace_formulas \<longrightarrow> (p \<Turnstile> \<phi> \<longleftrightarrow> q \<Turnstile> \<phi>))"
+proof
+  assume trace_eq: "traces p = traces q"
+  show "\<forall>\<phi>. \<phi> \<in> HML_trace_formulas \<longrightarrow> (p \<Turnstile> \<phi>) = (q \<Turnstile> \<phi>)"
+    using HM_trace_aux_theorem state_satisfies_trace trace_eq by blast
+next
+  assume assm: "(\<forall>\<phi>. \<phi> \<in> HML_trace_formulas \<longrightarrow> (p \<Turnstile> \<phi> \<longleftrightarrow> q \<Turnstile> \<phi>))"
+  show "traces p = traces q"
+    using state_satisfies_trace assm ttf ttf_in_HML_trace by blast
+qed
+
+section \<open>Hennessy–Milner Theorem of Modal Logic an Bisimilarity\<close>
+
+lemma hml_bisim_invariant:
+  assumes
+    \<open>p \<simeq>B q\<close>
+    \<open>p \<Turnstile> \<phi>\<close>
+  shows
+    \<open>q \<Turnstile> \<phi>\<close>
+  using assms
+proof (induct \<phi> arbitrary: p q)
+  case (HML_conj x1 x2)
+  then show ?case 
+    using bisimilar_def sympD by fastforce
+next
+  case (HML_poss x1 \<phi>)
+  then show ?case using simulation_def
+    by (metis bisim_sim local.HML_sem_poss)
+qed
+
+lemma HML_equiv_sim:
+  assumes "image_finite"
+  shows \<open>simulation HML_equivalent\<close>
+  unfolding simulation_def
+proof (safe, rule ccontr)
+  fix p q a p'
+define \<phi>d_set where
+  \<open>\<phi>d_set \<equiv> {SOME \<psi>. distinguishes \<psi> p' q' | q'. q' \<in> derivatives q a}\<close>
+  from assms have "finite (derivatives q a)" unfolding image_finite_def
+    by blast
+  then have "finite \<phi>d_set" unfolding \<phi>d_set_def
+    by simp
+  define \<phi>d where
+\<open>\<phi>d \<equiv> HML_poss a (HML_conj [] [])\<close>
+    \<open>\<phi>d \<equiv> HML_conj (derivatives q a) (\<lambda>q'. SOME \<phi>. distinguishes \<phi> p' q')\<close>
+  assume contra_assms:
+    \<open>p \<mapsto> a p'\<close> \<open>HML_equivalent p q\<close> \<open>\<nexists>q'. q \<mapsto> a q' \<and>  HML_equivalent p' q'\<close>
+  hence \<open>\<forall>q' \<in> derivatives q a. \<exists>\<phi>. distinguishes \<phi> p' q'\<close>
+    using hml_distinctions by simp
+  hence \<open>p' \<Turnstile> \<phi>d \<and> (\<forall>q' \<in> derivatives q a. \<not>q' \<Turnstile> \<phi>d)\<close>
+    unfolding \<phi>d_def by auto (smt (verit, best) someI2_ex)+
+  with contra_assms(1) have \<open>distinguishes (\<langle>a\<rangle>\<phi>d) p q\<close> by auto
+  thus False using contra_assms unfolding HML_equivalent_def by blast
+qed
+
+theorem Hennessy_Milner_theorem:
+  shows
+    \<open>HML_equivalent p q = (p \<simeq>B q)\<close>
+  using hml_bisim_invariant hml_equiv_sym HML_equiv_sim hml_distinctions
+  unfolding bisimilar_def HML_equivalent_def by blast
+
+
+
+end
+end
